
BOOLEAN ALGEBRA

Boolean Algebra

- ◇ A Boolean algebra is a closed algebraic system containing a set K of two or more elements and the two operators \cdot and $+$ which refer to logical AND and logical OR.

Basic Identities

$$(1) \ x + 0 = x$$

$$(3) \ x + 1 = 1$$

$$(5) \ x + x = x$$

$$(7) \ x + x' = 1$$

$$(2) \ x \cdot 0 = 0$$

$$(4) \ x \cdot 1 = x$$

$$(6) \ x \cdot x = x$$

$$(8) \ x \cdot x' = 0$$

Basic Identities

◇ Commutative Law

$$9. \quad x \bullet y = y \bullet x$$

$$10. \quad x + y = y + x$$

◇ Associative Law

$$11. \quad x \bullet (y \bullet z) = (x \bullet y) \bullet z$$

$$12. \quad x + (y + z) = (x + y) + z$$

◇ Distributive

$$13. x \bullet (y+z) = xy + xz$$

$$14. x + (y \bullet z) = (x + y)(x + z)$$

◇ Involution

$$15. (x')' = x$$

Duality

- ◇ A true Boolean Algebra expression can be converted into another true Boolean algebra expression by making the following substitutions:

$$1 \leftrightarrow 0$$

$$\bullet \leftrightarrow +$$

DeMorgan's Theorem

- ◇ **DeMorgan's Theorem provides the final link in taking any expression, including an expression with NAND or NOR, and converting it to S-o-P or P-o-S form.**

$$16. (x+y)' = x' \bullet y'$$

$$17. (x \bullet y)' = x' + y'$$

Function Minimization using Boolean Algebra

Examples:



$$***a + ab***$$

$$**= a(1+b) \text{ (Identity - 3)}**$$

$$**= a**$$



$$**a(a + b)**$$

$$**= a.a + ab \text{ (Distributive Law)}**$$

$$**= a+ab**$$

$$**= a(1+b) \text{ (Identity - 3)}**$$

$$**= a**$$

◇ $a + a'b$
= $(a + a')(a + b)$ (**Distributive Law**)
= $1(a + b)$
= $a + b$

◇ $a(a' + b)$
= $a \cdot a' + ab$ (*Distributive Law*)
= $0 + ab$
= ab

Show That

1. $ab + ab' = a$

2. $(a + b)(a + b') = a$

◇ **$ab + ab' = a$**

L.H.S = $ab + ab'$

= $a(b+b')$

= $a(1)$

= a

= R.H.S

$$\diamond (a + b)(a + b') = a$$

$$\text{L.H.S.} = (a+b)(a+b')$$

$$= a + (b*b') \text{ (Distributive Law)}$$

$$= a + (0) \text{ (Identity - 8)}$$

$$= a + 0$$

$$= a \text{ (Identity - 1)}$$

$$= \text{R.H.S.}$$